lib/loops: Split array definitions out of Loops.v

src/Rupicola/Lib/Loops.v
@@ -1,30 +1,5 @@
-Require Coq.Vectors.Vector.
-Require Import Arith PeanoNat.
-Require Import Coq.Program.Wf.
-Require Import Coq.Setoids.Setoid.
-Require Import Coq.derive.Derive.
-Require Import Coq.funind.Recdef.
-Require Import Coq.micromega.Psatz.
-
-Require coqutil.Map.SortedListString.
-
+From Coq Require Recdef.
 Require Import Rupicola.Lib.Api.
-Require Import Rupicola.Examples.Cells.Cells.
-
-(* (* Set Primitive Projections. *) *)
-(* Record p2 {A B} := P2 { pfst: A; psnd: B }. *)
-(* (* Unset Primitive Projections. *) *)
-(* Arguments P2 {A B} pfst psnd: assert. *)
-(* Arguments p2: clear implicits. *)
-
-Lemma extends_refl {p o} {map: map.map p o} m:
-  map.extends m m.
-Proof. firstorder. Qed.
-
-Lemma extends_eq {p o} {map: map.map p o} m1 m2:
-  m1 = m2 ->
-  map.extends m1 m2.
-Proof. intros * ->; apply extends_refl. Qed.
 
 Module Type ExitToken_sig.
   Axiom t : Set.
@@ -41,47 +16,6 @@ Module ExitToken <: ExitToken_sig.
   Definition branch {A} (tok: t) (set unset: A) :=
     if tok then set else unset.
 End ExitToken.
-
-Class HasDefault (T: Type) := default: T.
-
-Class Convertible (T1 T2: Type) := cast: T1 -> T2.
-
-Module VectorArray.
-  Section VectorArray.
-    Context {K V: Type}.
-    Context {Conv: Convertible K nat}.
-
-    Definition t n := Vector.t V n.
-    Definition get {n} (a: t n) (k: K) (pr: cast k < n) : V :=
-      Vector.nth_order a pr.
-    Definition put {n} (a: t n) (k: K) (pr: cast k < n) (v: V) : t n :=
-      Vector.replace_order a pr v.
-    (* FIXME needs an accessor that generates a test and returns a default *)
-  End VectorArray.
-
-  Arguments t : clear implicits.
-End VectorArray.
-
-Module ListArray.
-  Section ListArray.
-    Context {K V: Type}.
-    Context {HD: HasDefault V}.
-    Context {Conv: Convertible K nat}.
-
-    Definition t := list V.
-    Definition get (a: t) (k: K) : V :=
-      List.nth (cast k) a default.
-    Definition put (a: t) (k: K) (v: V) : t :=
-      replace_nth (cast k) a v.
-    (* FIXME needs an accessor that generates a test and returns a default *)
-
-    Lemma put_length (a: t) (k: K) (v: V) :
-      List.length (put a k v) = List.length a.
-    Proof. intros; apply replace_nth_length. Qed.
-  End ListArray.
-
-  Arguments t : clear implicits.
-End ListArray.
 
 Section Gallina.
   Open Scope Z_scope.
@@ -275,617 +209,6 @@ Section with_parameters.
   Context {semantics : Semantics.parameters}
           {semantics_ok : Semantics.parameters_ok semantics}.
 
-  Section WordArray.
-    Context
-      {A K} (to_list: A -> list word) (to_word: K -> word)
-      (get: A -> K -> word)
-      (put: A -> K -> word -> A)
-      (repr: address -> A -> Semantics.mem -> Prop).
-
-    Notation to_nat idx := (Z.to_nat (word.unsigned (to_word idx))).
-
-    Context (a : A) (a_ptr : word) (a_var : string)
-            (val: word) (val_var: string)
-            (idx : K) (idx_var : string).
-
-    Context
-      (Hget: forall a,
-         exists default,
-           get a idx =
-           List.hd default (List.skipn (to_nat idx) (to_list a)))
-      (Hput:
-         (to_nat idx < List.length (to_list a))%nat ->
-         to_list (put a idx val) =
-         List.app
-           (List.firstn (to_nat idx) (to_list a))
-           (val :: List.skipn (S (to_nat idx)) (to_list a)))
-      (Hgetput:
-         (to_nat idx < List.length (to_list a))%nat ->
-         get (put a idx val) idx = val)
-      (Hrw:
-         Lift1Prop.iff1
-           (repr a_ptr a)
-           (array scalar (word.of_Z (Memory.bytes_per_word Semantics.width))
-                  a_ptr (to_list a)))
-      (Hrw_put:
-         Lift1Prop.iff1
-           (repr a_ptr (put a idx val))
-           (array scalar (word.of_Z (Memory.bytes_per_word Semantics.width))
-                  a_ptr (to_list (put a idx val)))).
-
-    Lemma compile_word_array_get {tr mem locals functions}:
-      let v := get a idx in
-      forall {P} {pred: P v -> predicate} {k: nlet_eq_k P v} {k_impl : cmd}
-        R (var : string),
-
-        (Z.to_nat (word.unsigned (to_word idx)) < Datatypes.length (to_list a))%nat ->
-
-        sep (repr a_ptr a) R mem ->
-        map.get locals a_var = Some a_ptr ->
-        map.get locals idx_var = Some (to_word idx) ->
-
-        (let v := v in
-         <{ Trace := tr;
-            Memory := mem;
-            Locals := map.put locals var v;
-            Functions := functions }>
-         k_impl
-         <{ pred (k v eq_refl) }>) ->
-        <{ Trace := tr;
-           Memory := mem;
-           Locals := locals;
-           Functions := functions }>
-        cmd.seq
-          (cmd.set
-             var
-             (expr.load
-                access_size.word
-                (expr.op bopname.add
-                         (expr.var a_var)
-                         (expr.op bopname.mul
-                                  (expr.literal (Memory.bytes_per_word Semantics.width))
-                                  (expr.var idx_var)))))
-          k_impl
-        <{ pred (nlet_eq [var] v k) }>.
-    Proof.
-      cbn; intros Hlt *.
-      pose proof word.unsigned_range (to_word idx) as (Hge & _).
-      destruct (Hget a) as [default Hget0].
-
-      exists (get a idx); split; cbn; [ | assumption ].
-      exists a_ptr; split; [ eassumption | ]; cbn.
-      exists (to_word idx); split; [ eassumption | ]; cbn.
-      eexists; split; [ | reflexivity ].
-
-      eapply load_word_of_sep.
-      seprewrite_in Hrw H0.        (* FIXME seprewrite shouldn't rename *)
-      (* FIXME: BEDROCK2: Adding an extra "_" at the end shelves an inequality *)
-      once (seprewrite_in open_constr:(array_index_nat_inbounds
-                                         _ _ _ _ (Z.to_nat (word.unsigned (to_word idx)))) H5).
-      { assumption. }
-
-      rewrite word.ring_morph_mul, Z2Nat.id, !word.of_Z_unsigned in H4 by assumption.
-      rewrite Hget0.
-      ecancel_assumption.
-    Qed.
-
-    Lemma compile_word_array_put {tr mem locals functions} :
-      let v := put a idx val in
-      forall {P} {pred: P v -> predicate} {k: nlet_eq_k P v} {k_impl: cmd}
-        R (var: string),
-
-      (Z.to_nat (word.unsigned (to_word idx)) < Datatypes.length (to_list a))%nat ->
-
-      sep (repr a_ptr a) R mem ->
-      map.get locals a_var = Some a_ptr ->
-      map.get locals idx_var = Some (to_word idx) ->
-      map.get locals val_var = Some val ->
-
-      (let v := v in
-       forall mem',
-         sep (repr a_ptr v) R mem' ->
-         <{ Trace := tr;
-            Memory := mem';
-            Locals := locals;
-            Functions := functions }>
-         k_impl
-         <{ pred (k v eq_refl) }>) ->
-      <{ Trace := tr;
-         Memory := mem;
-         Locals := locals;
-         Functions := functions }>
-      cmd.seq
-        (cmd.store
-           access_size.word
-           (expr.op bopname.add
-                    (expr.var a_var)
-                    (expr.op bopname.mul
-                             (expr.literal (Memory.bytes_per_word Semantics.width))
-                             (expr.var idx_var)))
-           (expr.var val_var))
-        k_impl
-      <{ pred (nlet_eq [var] v k) }>.
-    Proof.
-      cbn; intros Hlt *.
-      pose proof word.unsigned_range (to_word idx) as (Hge & _).
-      destruct (Hget (put a idx val)) as [default Hget0].
-      eexists; split; cbn.
-
-      { eexists; split; [ eassumption | ]; cbn.
-        eexists; split; [ eassumption | reflexivity ]. }
-
-      { eexists; split; cbn.
-        { eexists; split; [ eassumption | reflexivity ]. }
-        { seprewrite_in Hrw H0.
-          once (seprewrite_in
-                  open_constr:(array_index_nat_inbounds
-                                 _ _ (default := default) _ _ (Z.to_nat (word.unsigned (to_word idx)))) H6).
-          { assumption. }
-
-          eapply store_word_of_sep.
-          { rewrite word.ring_morph_mul, Z2Nat.id, !word.of_Z_unsigned in H5 by assumption.
-            ecancel_assumption. }
-          { intros m Hm.
-            apply H4.
-            seprewrite Hrw_put.
-            seprewrite
-              open_constr:(array_index_nat_inbounds
-                             _ _ (default := default) _ _ (Z.to_nat (word.unsigned (to_word idx)))).
-            { rewrite Hput by lia.
-              rewrite List.app_length, List.firstn_length_le by lia.
-              cbn [List.length]; rewrite List.length_skipn.
-              lia. }
-            { rewrite <- Hget0, Hgetput by lia.
-              repeat rewrite word.ring_morph_mul, Z2Nat.id, !word.of_Z_unsigned by lia.
-              rewrite Hput by lia.
-
-              rewrite List.firstn_app.
-              rewrite List.firstn_firstn, Min.min_idempotent.
-              rewrite List.firstn_length_le by lia.
-              rewrite Nat.sub_diag; cbn [List.firstn]; rewrite app_nil_r.
-
-              change (val :: ?tl) with (List.app [val] tl).
-              rewrite List.app_assoc, List.skipn_app, List.skipn_all, List.app_nil_l, List.skipn_skipn;
-                rewrite !List.app_length, List.firstn_length_le, (Nat.add_comm _ 1) by lia.
-              - rewrite Nat.sub_diag, Nat.add_0_l.
-                ecancel_assumption.
-              - reflexivity. } } } }
-    Qed.
-  End WordArray.
-
-  Instance Convertible_word_Nat : Convertible word nat :=
-    fun w => Z.to_nat (word.unsigned w).
-  Instance HasDefault_word : HasDefault word :=
-    word.of_Z 0.
-
-  Section WordVectorArray.
-    Definition word_vectorarray_value {n} (addr: address) (a: VectorArray.t word n) : Semantics.mem -> Prop :=
-      array scalar (word.of_Z (Memory.bytes_per_word Semantics.width)) addr (Vector.to_list a).
-
-    Notation repr := word_vectorarray_value.
-    Notation to_list := Vector.to_list.
-    Notation to_word := (proj1_sig (P:=fun idx0 : word => (cast idx0 < _)%nat)).
-    Notation to_nat idx := (Z.to_nat (word.unsigned (to_word idx))).
-
-    Notation get a idx := (VectorArray.get a (proj1_sig idx) (proj2_sig idx)).
-    Notation put a idx v := (VectorArray.put a (proj1_sig idx) (proj2_sig idx) v).
-
-    Lemma WordVectorArray_Hget {n}:
-      forall (a: VectorArray.t word n) idx,
-      exists default,
-        get a idx =
-        List.hd default (List.skipn (to_nat idx) (to_list a)).
-    Proof.
-      intros. exists (word.of_Z 0).
-      apply Vector_nth_hd_skipn.
-      rewrite Fin.to_nat_of_nat; reflexivity.
-    Qed.
-
-    Lemma WordVectorArray_Hput {n} :
-      forall (a : VectorArray.t word n) (idx: {idx : word | (cast idx < n)%nat}) v,
-        to_list (put a idx v) =
-        List.app
-          (List.firstn (to_nat idx) (to_list a))
-          (v :: List.skipn (S (to_nat idx)) (to_list a)).
-    Proof.
-      unfold put.
-      destruct idx as [widx pr]; cbn [proj1_sig proj2_sig].
-      unfold cast, Convertible_word_Nat in *.
-      set (Z.to_nat (word.unsigned widx)) as idx in *.
-      intros.
-      unfold Vector.replace_order; erewrite Vector_to_list_replace by reflexivity.
-      rewrite <- replace_nth_eqn by (rewrite Vector_to_list_length; assumption).
-      rewrite Fin.to_nat_of_nat; reflexivity.
-    Qed.
-
-    Lemma WordVectorArray_Hgetput {n} :
-      forall (a : VectorArray.t word n) (idx: {idx : word | (cast idx < n)%nat}) v,
-        get (put a idx v) idx = v.
-    Proof.
-      unfold get, put, Vector.nth_order, Vector.replace_order.
-      intros; apply Vector_nth_replace.
-    Qed.
-
-    Lemma WordVectorArray_Hrw {n}:
-      forall addr (a: VectorArray.t word n),
-        Lift1Prop.iff1
-          (repr addr a)
-          (array scalar (word.of_Z (Memory.bytes_per_word Semantics.width))
-                 addr (to_list a)).
-    Proof. reflexivity. Qed.
-
-    Lemma compile_word_vectorarray_get {n} {tr mem locals functions}
-          (a: VectorArray.t word n) idx pr:
-      let v := VectorArray.get a idx pr in
-      forall {P} {pred: P v -> predicate} {k: nlet_eq_k P v} {k_impl}
-        R (a_ptr: address) a_var idx_var var,
-
-        sep (word_vectorarray_value a_ptr a) R mem ->
-        map.get locals a_var = Some a_ptr ->
-        map.get locals idx_var = Some idx ->
-
-        (let v := v in
-         <{ Trace := tr;
-            Memory := mem;
-            Locals := map.put locals var v;
-            Functions := functions }>
-         k_impl
-         <{ pred (k v eq_refl) }>) ->
-        <{ Trace := tr;
-           Memory := mem;
-           Locals := locals;
-           Functions := functions }>
-        cmd.seq
-          (cmd.set
-             var
-             (expr.load
-                access_size.word
-                (expr.op bopname.add
-                         (expr.var a_var)
-                         (expr.op bopname.mul
-                                  (expr.literal (Memory.bytes_per_word Semantics.width))
-                                  (expr.var idx_var)))))
-          k_impl
-        <{ pred (nlet_eq [var] v k) }>.
-    Proof.
-      intros.
-      change v with
-          ((fun a idx => VectorArray.get a (proj1_sig idx) (proj2_sig idx))
-             a (exist (fun idx => cast idx < n)%nat idx pr)).
-      eapply (compile_word_array_get to_list to_word);
-        eauto using WordVectorArray_Hget, WordVectorArray_Hrw.
-      { rewrite Vector_to_list_length.
-        simpl. assumption. }
-    Qed.
-
-    Lemma compile_word_vectorarray_put {n} {tr mem locals functions}
-          (a: VectorArray.t word n) idx pr val:
-      let v := VectorArray.put a idx pr val in
-      forall {P} {pred: P v -> predicate} {k: nlet_eq_k P v} {k_impl}
-        R a_ptr a_var idx_var val_var var,
-
-        sep (word_vectorarray_value a_ptr a) R mem ->
-        map.get locals a_var = Some a_ptr ->
-        map.get locals idx_var = Some idx ->
-        map.get locals val_var = Some val ->
-
-        (let v := v in
-         forall mem',
-           sep (word_vectorarray_value a_ptr v) R mem' ->
-           <{ Trace := tr;
-              Memory := mem';
-              Locals := locals;
-              Functions := functions }>
-           k_impl
-           <{ pred (k v eq_refl) }>) ->
-        <{ Trace := tr;
-           Memory := mem;
-           Locals := locals;
-           Functions := functions }>
-        cmd.seq
-          (cmd.store
-             access_size.word
-             (expr.op bopname.add
-                      (expr.var a_var)
-                      (expr.op bopname.mul
-                               (expr.literal (Memory.bytes_per_word Semantics.width))
-                               (expr.var idx_var)))
-             (expr.var val_var))
-          k_impl
-        <{ pred (nlet_eq [var] v k) }>.
-    Proof.
-      intros.
-      change v with
-          ((fun v idx val => VectorArray.put a (proj1_sig idx) (proj2_sig idx) val)
-             v (exist (fun idx => cast idx < n)%nat idx pr) val).
-      eapply (compile_word_array_put
-                to_list to_word
-                (fun a idx => get a idx)
-                (fun a idx v => put a idx v));
-        eauto using WordVectorArray_Hget, WordVectorArray_Hrw,
-        WordVectorArray_Hgetput, WordVectorArray_Hput.
-      rewrite Vector_to_list_length; assumption.
-    Qed.
-  End WordVectorArray.
-
-  Section WordListArray.
-    Definition word_listarray_value (addr: address) (a: ListArray.t word)
-      : Semantics.mem -> Prop :=
-      array scalar (word.of_Z (Memory.bytes_per_word Semantics.width)) addr a.
-
-    Notation repr := word_listarray_value.
-    Notation to_list x := x (only parsing).
-    Notation to_word x := x (only parsing).
-    Notation to_nat idx := (Z.to_nat (word.unsigned (to_word idx))).
-
-    Notation get a idx := (ListArray.get a idx).
-    Notation put a idx v := (ListArray.put a idx v).
-
-    Lemma WordListArray_Hget:
-      forall (a: ListArray.t word) idx,
-      exists default,
-        get a idx =
-        List.hd default (List.skipn (to_nat idx) (to_list a)).
-    Proof.
-      intros. exists (word.of_Z 0).
-      unfold get; rewrite <- List.nth_default_eq.
-      apply List.hd_skipn_nth_default.
-    Qed.
-
-    Lemma WordListArray_Hput :
-      forall (a : ListArray.t word) (idx: word) v,
-        (to_nat idx < Datatypes.length a)%nat ->
-        to_list (put a idx v) =
-        List.app
-          (List.firstn (to_nat idx) (to_list a))
-          (v :: List.skipn (S (to_nat idx)) (to_list a)).
-    Proof.
-      unfold put; eauto using replace_nth_eqn.
-    Qed.
-
-    Lemma WordListArray_Hgetput :
-      forall (a : ListArray.t word) (idx: word) v,
-        (to_nat idx < Datatypes.length a)%nat ->
-        get (put a idx v) idx = v.
-    Proof.
-      unfold get, put.
-      intros; apply nth_replace_nth; (assumption || reflexivity).
-    Qed.
-
-    Lemma WordListArray_Hrw:
-      forall addr (a: ListArray.t word),
-        Lift1Prop.iff1
-          (repr addr a)
-          (array scalar (word.of_Z (Memory.bytes_per_word Semantics.width))
-                 addr (to_list a)).
-    Proof. reflexivity. Qed.
-
-    Lemma compile_word_listarray_get {tr mem locals functions}
-          (a: ListArray.t word) idx:
-      let v := ListArray.get a idx in
-      forall {P} {pred: P v -> predicate} {k: nlet_eq_k P v} {k_impl}
-        R (a_ptr: address) a_var idx_var var,
-
-        sep (word_listarray_value a_ptr a) R mem ->
-        map.get locals a_var = Some a_ptr ->
-        map.get locals idx_var = Some idx ->
-
-        word.unsigned idx < Z.of_nat (Datatypes.length (id a)) ->
-
-        (let v := v in
-         <{ Trace := tr;
-            Memory := mem;
-            Locals := map.put locals var v;
-            Functions := functions }>
-         k_impl
-         <{ pred (k v eq_refl) }>) ->
-        <{ Trace := tr;
-           Memory := mem;
-           Locals := locals;
-           Functions := functions }>
-        cmd.seq
-          (cmd.set
-             var
-             (expr.load
-                access_size.word
-                (expr.op bopname.add
-                         (expr.var a_var)
-                         (expr.op bopname.mul
-                                  (expr.literal (Memory.bytes_per_word Semantics.width))
-                                  (expr.var idx_var)))))
-          k_impl
-        <{ pred (nlet_eq [var] v k) }>.
-    Proof.
-      intros.
-      eapply (compile_word_array_get id id);
-        eauto using WordListArray_Hget, WordListArray_Hrw.
-      pose proof word.unsigned_range idx.
-      unfold id in *; lia.
-    Qed.
-
-    Lemma compile_word_listarray_put {tr mem locals functions}
-          (a: ListArray.t word) idx val:
-      let v := ListArray.put a idx val in
-      forall {P} {pred: P v -> predicate} {k: nlet_eq_k P v} {k_impl}
-        R (a_ptr: address) a_var idx_var val_var var,
-
-        sep (word_listarray_value a_ptr a) R mem ->
-        map.get locals a_var = Some a_ptr ->
-        map.get locals idx_var = Some idx ->
-        map.get locals val_var = Some val ->
-
-        (word.unsigned idx < Z.of_nat (List.length a))%Z ->
-
-        (let v := v in
-         forall mem',
-           sep (word_listarray_value a_ptr v) R mem' ->
-           <{ Trace := tr;
-              Memory := mem';
-              Locals := locals;
-              Functions := functions }>
-           k_impl
-           <{ pred (k v eq_refl) }>) ->
-        <{ Trace := tr;
-           Memory := mem;
-           Locals := locals;
-           Functions := functions }>
-        cmd.seq
-          (cmd.store
-             access_size.word
-             (expr.op bopname.add
-                      (expr.var a_var)
-                      (expr.op bopname.mul
-                               (expr.literal (Memory.bytes_per_word Semantics.width))
-                               (expr.var idx_var)))
-             (expr.var val_var))
-          k_impl
-        <{ pred (nlet_eq [var] v k) }>.
-    Proof.
-      intros.
-      eapply (compile_word_array_put id id);
-        eauto using WordListArray_Hget, WordListArray_Hput,
-        WordListArray_Hgetput, WordListArray_Hrw.
-      unfold id; pose proof word.unsigned_range idx.
-      lia.
-    Qed.
-  End WordListArray.
-
-  Section WordSizedListArray.
-    Definition word_sizedlistarray_value (addr: address) (len: nat) (a: ListArray.t word)
-      : Semantics.mem -> Prop :=
-      sep (emp (List.length a = len)) (array scalar (word.of_Z (Memory.bytes_per_word Semantics.width)) addr a).
-
-    Notation repr := word_sizedlistarray_value.
-    Notation to_list x := x (only parsing).
-    Notation to_word x := x (only parsing).
-    Notation to_nat idx := (Z.to_nat (word.unsigned (to_word idx))).
-
-    Notation get a idx := (ListArray.get a idx).
-    Notation put a idx v := (ListArray.put a idx v).
-
-    Lemma WordSizedListArray_Hrw:
-      forall addr sz (a: ListArray.t word),
-        List.length a = sz ->
-        Lift1Prop.iff1
-          (repr addr sz a)
-          (array scalar (word.of_Z (Memory.bytes_per_word Semantics.width))
-                 addr (to_list a)).
-    Proof. unfold word_sizedlistarray_value.
-       intros. setoid_replace (Datatypes.length a = sz) with True.
-       - apply sep_emp_True_l.
-       - tauto.
-    Qed.
-
-    Lemma WordSizedListArray_length :
-      forall addr sz (a: ListArray.t word) mem R,
-        (repr addr sz a * R)%sep mem -> List.length a = sz.
-    Proof.
-      intros * H; unfold repr in H.
-      eapply proj1. apply sep_emp_l with (m := mem).
-      ecancel_assumption.
-    Qed.
-
-    Lemma compile_word_sizedlistarray_get {sz} {tr mem locals functions}
-          (a: ListArray.t word) idx:
-      let v := ListArray.get a idx in
-      forall {P} {pred: P v -> predicate} {k: nlet_eq_k P v} {k_impl}
-        R (a_ptr: address) a_var idx_var var,
-
-        sep (word_sizedlistarray_value a_ptr sz a) R mem ->
-        map.get locals a_var = Some a_ptr ->
-        map.get locals idx_var = Some idx ->
-
-        word.unsigned idx < Z.of_nat sz ->
-
-        (let v := v in
-         <{ Trace := tr;
-            Memory := mem;
-            Locals := map.put locals var v;
-            Functions := functions }>
-         k_impl
-         <{ pred (k v eq_refl) }>) ->
-        <{ Trace := tr;
-           Memory := mem;
-           Locals := locals;
-           Functions := functions }>
-        cmd.seq
-          (cmd.set
-             var
-             (expr.load
-                access_size.word
-                (expr.op bopname.add
-                         (expr.var a_var)
-                         (expr.op bopname.mul
-                                  (expr.literal (Memory.bytes_per_word Semantics.width))
-                                  (expr.var idx_var)))))
-          k_impl
-        <{ pred (nlet_eq [var] v k) }>.
-    Proof.
-      intros.
-      eapply (compile_word_array_get id id _ (fun addr a => repr addr sz a));
-        eauto using WordListArray_Hget.
-      - eapply WordSizedListArray_Hrw, WordSizedListArray_length.
-        eassumption.
-      - unfold id.
-        erewrite WordSizedListArray_length by eassumption.
-        pose proof word.unsigned_range idx.
-        lia.
-    Qed.
-
-    Lemma compile_word_sizedlistarray_put {sz} {tr mem locals functions}
-          (a: ListArray.t word) idx val:
-      let v := ListArray.put a idx val in
-      forall {P} {pred: P v -> predicate} {k: nlet_eq_k P v} {k_impl}
-        R (a_ptr: address) a_var idx_var val_var var,
-
-        sep (word_sizedlistarray_value a_ptr sz a) R mem ->
-        map.get locals a_var = Some a_ptr ->
-        map.get locals idx_var = Some idx ->
-        map.get locals val_var = Some val ->
-
-        (word.unsigned idx < Z.of_nat sz)%Z ->
-
-        (let v := v in
-         forall mem',
-           sep (word_sizedlistarray_value a_ptr sz v) R mem' ->
-           <{ Trace := tr;
-              Memory := mem';
-              Locals := locals;
-              Functions := functions }>
-           k_impl
-           <{ pred (k v eq_refl) }>) ->
-        <{ Trace := tr;
-           Memory := mem;
-           Locals := locals;
-           Functions := functions }>
-        cmd.seq
-          (cmd.store
-             access_size.word
-             (expr.op bopname.add
-                      (expr.var a_var)
-                      (expr.op bopname.mul
-                               (expr.literal (Memory.bytes_per_word Semantics.width))
-                               (expr.var idx_var)))
-             (expr.var val_var))
-          k_impl
-        <{ pred (nlet_eq [var] v k) }>.
-    Proof.
-      intros.
-      eapply (compile_word_array_put id id _ _ (fun (addr: word) a => repr addr sz a));
-        eauto using WordListArray_Hget, WordListArray_Hput,
-        WordListArray_Hgetput.
-      - eapply WordSizedListArray_Hrw, WordSizedListArray_length.
-        eassumption.
-      - eapply WordSizedListArray_Hrw.
-        unfold id; rewrite ListArray.put_length.
-        eapply WordSizedListArray_length.
-        eassumption.
-      - unfold id; pose proof word.unsigned_range idx.
-        erewrite WordSizedListArray_length by eassumption.
-        lia.
-    Qed.
-  End WordSizedListArray.
-
   Definition ranged_for_widen_bounds {from idx from' to} :
     from <= idx < from' ->
     from' < to ->
@@ -967,32 +290,20 @@ Section with_parameters.
 
   Definition compile_ranged_for_s :=
     compile_ranged_for_w word_signed_of_Z_bracketed.
+End with_parameters.
 
-  Hint Extern 1 => simple eapply compile_get; shelve : compiler.
-  Hint Extern 1 => simple eapply compile_put; shelve : compiler.
-  Hint Extern 1 => simple eapply compile_word_vectorarray_get; shelve : compiler.
-  Hint Extern 1 => simple eapply compile_word_vectorarray_put; shelve : compiler.
-  Hint Extern 1 => simple eapply compile_word_sizedlistarray_get; shelve : compiler.
-  Hint Extern 1 => simple eapply compile_word_sizedlistarray_put; shelve : compiler.
+Require Import Rupicola.Lib.Arrays.
+Require Import Rupicola.Examples.Cells.Cells.
+
+Section Ex.
+  Context {semantics : Semantics.parameters}
+          {semantics_ok : Semantics.parameters_ok semantics}.
 
    Notation "∅" := map.empty.
    Notation "m [[ k ← v ]]" :=
      (map.put m k v)
        (left associativity, at level 11,
         format "m [[ k  ←  v ]]").
-
-   Ltac try_unify x y :=
-     try ((unify x y; fail 1) || fail 1 "Does not unify").
-
-   Ltac lookup_variable m val ::=
-     match m with
-     | map.put _ ?k ?val' =>
-       let t := type of val in
-       let _ := constr:(@eq_refl t val <: val = val') in
-       constr:(k)
-     | map.put ?m' _ _ => lookup_variable m' val
-     | _ => fail "lookup_variable: no results found"
-     end.
 
    Lemma signed_lt_unsigned w:
      word.signed w <= word.unsigned w.
@@ -1001,6 +312,11 @@ Section with_parameters.
      rewrite word.signed_unsigned_dec.
      destruct Z_lt_le_dec; lia.
    Qed.
+
+  Instance Convertible_word_Nat : Convertible word nat :=
+    fun w => Z.to_nat (word.unsigned w).
+  Instance HasDefault_word : HasDefault word :=
+    word.of_Z 0.
 
     Program Definition vect_memcpy {n1 n2} (len: word)
            (a1: VectorArray.t word n1)
@@ -1029,24 +345,21 @@ Section with_parameters.
       lia.
     Qed.
 
-   Definition TwoVectArrays {n1 n2} a1_ptr a2_ptr :=
-     (fun '(a1, a2) (_retvals: list word) =>
-        (word_vectorarray_value (n := n1) a1_ptr a1 *
-         word_vectorarray_value (n := n2) a2_ptr a2)%sep).
-   Hint Unfold TwoVectArrays : compiler_cleanup.
-
    Instance spec_of_vect_memcpy : spec_of "vect_memcpy" :=
-     (forall! (len: word) (a1_ptr a2_ptr : address)
-       {n1} (a1: VectorArray.t word n1)
-       {n2} (a2: VectorArray.t word n2)
-       (pr1: word.unsigned len < Z.of_nat n1)
-       (pr2: word.unsigned len < Z.of_nat n2),
-         (fun R mem =>
-            sep (word_vectorarray_value a1_ptr a1 * word_vectorarray_value a2_ptr a2)%sep R mem)
-         ===>
-         "vect_memcpy" @ [len; a1_ptr; a2_ptr]
-         ===>
-         (TwoVectArrays a1_ptr a2_ptr (vect_memcpy len a1 a2 pr1 pr2))).
+     fnspec "vect_memcpy" (len: word) (a1_ptr a2_ptr : address) /
+            {n1} (a1: VectorArray.t word n1)
+            {n2} (a2: VectorArray.t word n2)
+            (pr1: word.unsigned len < Z.of_nat n1)
+            (pr2: word.unsigned len < Z.of_nat n2)
+            R,
+     { requires tr mem :=
+         (word_vectorarray_value a1_ptr a1 ⋆
+          word_vectorarray_value a2_ptr a2 ⋆ R) mem;
+       ensures tr' mem' :=
+         tr' = tr /\
+         let res := vect_memcpy len a1 a2 pr1 pr2 in
+         (word_vectorarray_value a1_ptr (fst res) ⋆
+          word_vectorarray_value a2_ptr (snd res) ⋆ R) mem' }.
 
    Derive vect_memcpy_body SuchThat
           (defn! "vect_memcpy"("len", "a1", "a2") { vect_memcpy_body },
@@ -1061,184 +374,8 @@ Section with_parameters.
      eapply compile_ranged_for_u with (loop_pred := (fun idx a2 tr' mem' locals' =>
          tr' = tr /\
          locals' = (∅[["len" ← len]][["a1" ← a1_ptr]][["a2" ← a2_ptr]]
-                     [["from" ← idx]][["step" ← v0]]) /\
+                     [["from" ← idx]][["step" ← word.of_Z 1]]) /\
          (word_vectorarray_value a1_ptr a1 * word_vectorarray_value a2_ptr a2 * R)%sep mem')).
-
-     all: repeat compile_step; compile_done.
-   Qed.
-
-   Definition sizedlist_memcpy (len: word)
-           (a1: ListArray.t word)
-           (a2: ListArray.t word) :=
-     let/n from := word.of_Z 0 in
-     let/n step := word.of_Z 1 in
-     let/n a2 := ranged_for_u
-                  from len step
-                  (fun tok idx a2 Hlt =>
-                     let/n v := ListArray.get a1 idx in
-                     let/n a2 := ListArray.put a2 idx v in
-                     (tok, a2)) a2 in
-     (a1, a2).
-
-   Definition TwoSizedListArrays n1 n2 a1_ptr a2_ptr :=
-     (fun '(a1, a2) (_retvals: list word) =>
-        (word_sizedlistarray_value a1_ptr n1 a1 *
-         word_sizedlistarray_value a2_ptr n2 a2)%sep).
-   Hint Unfold TwoSizedListArrays : compiler_cleanup.
-
-   Instance spec_of_sizedlist_memcpy : spec_of "sizedlist_memcpy" :=
-     (forall! (len: word) (a1_ptr a2_ptr : address)
-       {n1} (a1: ListArray.t word)
-       {n2} (a2: ListArray.t word)
-       (pr1: word.unsigned len < Z.of_nat n1)
-       (pr2: word.unsigned len < Z.of_nat n2),
-         (fun R mem =>
-            sep (word_sizedlistarray_value a1_ptr n1 a1 *
-                 word_sizedlistarray_value a2_ptr n2 a2)%sep R mem)
-         ===>
-         "sizedlist_memcpy" @ [len; a1_ptr; a2_ptr]
-         ===>
-         (TwoSizedListArrays n1 n2 a1_ptr a2_ptr (sizedlist_memcpy len a1 a2))).
-
-   Derive sizedlist_memcpy_body SuchThat
-         (defn! "sizedlist_memcpy"("len", "a1", "a2") { sizedlist_memcpy_body },
-          implements sizedlist_memcpy)
-         As sizedlist_memcpy_correct.
-   Proof.
-     compile_setup.
-
-     repeat compile_step.
-
-     simple apply compile_nlet_as_nlet_eq.
-     eapply compile_ranged_for_u with (loop_pred := (fun idx a2 tr' mem' locals' =>
-         tr' = tr /\
-         locals' = (∅[["len" ← len]][["a1" ← a1_ptr]][["a2" ← a2_ptr]]
-                     [["from" ← idx]][["step" ← v0]]) /\
-         (word_sizedlistarray_value a1_ptr n1 a1 *
-          word_sizedlistarray_value a2_ptr n2 a2 * R)%sep mem')).
-
-     all: repeat compile_step; try lia; compile_done.
-   Qed.
-
-   Definition unsizedlist_memcpy (len: word)
-           (a1: ListArray.t word)
-           (a2: ListArray.t word) :=
-     let/n from := word.of_Z 0 in
-     let/n step := word.of_Z 1 in
-     let/n a2 := ranged_for_u
-                  from len step
-                  (fun tok idx a2 Hlt =>
-                     let/n v := ListArray.get a1 idx in
-                     let/n a2 := ListArray.put a2 idx v in
-                     (tok, a2)) a2 in
-     (a1, a2).
-
-   Definition TwoUnsizedListArrays a1_ptr a2_ptr :=
-     (fun '(a1, a2) (_retvals: list word) =>
-        (word_listarray_value a1_ptr a1 *
-         word_listarray_value a2_ptr a2)%sep).
-   Hint Unfold TwoUnsizedListArrays : compiler_cleanup.
-
-   Instance spec_of_unsizedlist_memcpy : spec_of "unsizedlist_memcpy" :=
-     (forall! (len: word) (a1_ptr a2_ptr : address)
-       (a1: ListArray.t word) (a2: ListArray.t word)
-       (pr1: word.unsigned len < Z.of_nat (List.length a1))
-       (pr2: word.unsigned len < Z.of_nat (List.length a2)),
-         (fun R mem =>
-            sep (word_listarray_value a1_ptr a1 *
-                 word_listarray_value a2_ptr a2)%sep R mem)
-         ===>
-         "unsizedlist_memcpy" @ [len; a1_ptr; a2_ptr]
-         ===>
-         (TwoUnsizedListArrays a1_ptr a2_ptr (unsizedlist_memcpy len a1 a2))).
-
-   Derive unsizedlist_memcpy_body SuchThat
-         (defn! "unsizedlist_memcpy"("len", "a1", "a2") { unsizedlist_memcpy_body },
-          implements unsizedlist_memcpy)
-         As unsizedlist_memcpy_correct.
-   Proof.
-     compile_setup.
-
-     repeat compile_step.
-
-     simple apply compile_nlet_as_nlet_eq.
-     eapply compile_ranged_for_u with (loop_pred := (fun idx a2 tr' mem' locals' =>
-         tr' = tr /\
-         locals' = (∅[["len" ← len]][["a1" ← a1_ptr]][["a2" ← a2_ptr]]
-                     [["from" ← idx]][["step" ← v0]]) /\
-         (word_listarray_value a1_ptr a1 *
-          word_listarray_value a2_ptr a2 * R)%sep mem')).
-
-     (*  FIXME remove previous hints *)
-     Hint Extern 1 => simple eapply compile_word_listarray_get; shelve : compiler.
-     Hint Extern 1 => simple eapply compile_word_listarray_put; shelve : compiler.
-
-     all: repeat compile_step; compile_done; unfold id.
-
-     { lia. (* loop index in bounds + function precondition *) }
-     { (* Note the call to induction.
-          Without vectors or the sizedlist predicate, we need to check that the index is in bounds but we modified the array.
-          Using a vector type instead keeps the information in the type and the statement of put specifies that the length is preserved.
-          Putting that info in the representation predicates has a similar effect.
-          Without this, we need to perform induction explicitly. *)
-       subst a.
-       apply ranged_for_u_ind.
-       - lia.
-       - intros; unfold nlet; cbn.
-         rewrite ListArray.put_length.
-         assumption. }
-   Qed.
-
-   Program Definition incr_gallina_spec (c: cell) : cell :=
-     let/n one := word.of_Z 1 in
-     let/n from := word.of_Z 3 in
-     let/n to := word.of_Z 5 in
-     let/n step := word.of_Z 1 in
-     let/n tick := word.of_Z 0 in
-     let/n (tick, c) :=
-        ranged_for_u (A := word * cell)
-                     from to step
-                     (fun tok idx acc bounded =>
-                        let '(tick, c) := acc in
-                        let/n v := get c in
-                        let/n v := word.add v idx in
-                        let/n c := put v c in
-                        let/n tick := word.add tick one in
-                        (tok, (tick, c)))
-                     (tick, c) : word * cell in
-     (let/n v := get c in
-      let/n v := word.add v tick in
-      let/n c := put v c in
-      c).
-
-  Print incr_gallina_spec.
-
-  Instance spec_of_incr : spec_of "incr" :=
-    (forall! (c_ptr : address) (c :cell),
-        (sep (cell_value c_ptr c))
-          ===>
-          "incr" @ [c_ptr]
-          ===>
-          (OneCell c_ptr (incr_gallina_spec c))).
-
-   Derive incr_body SuchThat
-         (defn! "incr"("c") { incr_body },
-          implements incr_gallina_spec)
-         As body_correct.
-   Proof.
-     compile_setup.
-
-     repeat compile_step.
-
-     simple apply compile_nlet_as_nlet_eq.
-     eapply compile_ranged_for_u with (loop_pred := (fun idx acc tr' mem' locals' =>
-         let '(tick, c) := acc in
-         tr' = tr /\
-         (* locals' = map.put locals "tick" tick /\ *)
-         locals' = (∅[["c" ← c_ptr]][["one" ← v]]
-                     [["from" ← idx]][["to" ← v1]][["step" ← v2]]
-                     [["tick" ← tick]]) /\
-         (cell_value c_ptr c * R)%sep mem')).
 
      all: repeat compile_step; compile_done.
    Qed.
@@ -1270,18 +407,22 @@ Section with_parameters.
      rewrite word.signed_gz_eq_unsigned; lia.
    Qed.
 
+
    Instance spec_of_vect_memcpy_s : spec_of "vect_memcpy_s" :=
-     (forall! (len: word) (a1_ptr a2_ptr : address)
-       {n1} (a1: VectorArray.t word n1)
-       {n2} (a2: VectorArray.t word n2)
-       (pr1: word.signed len < Z.of_nat n1)
-       (pr2: word.signed len < Z.of_nat n2),
-         (fun R mem =>
-            sep (word_vectorarray_value a1_ptr a1 * word_vectorarray_value a2_ptr a2)%sep R mem)
-         ===>
-         "vect_memcpy_s" @ [len; a1_ptr; a2_ptr]
-         ===>
-         (TwoVectArrays a1_ptr a2_ptr (vect_memcpy_s len a1 a2 pr1 pr2))).
+     fnspec "vect_memcpy_s" (len: word) (a1_ptr a2_ptr : address) /
+            {n1} (a1: VectorArray.t word n1)
+            {n2} (a2: VectorArray.t word n2)
+            (pr1: word.signed len < Z.of_nat n1)
+            (pr2: word.signed len < Z.of_nat n2)
+            R,
+     { requires tr mem :=
+         (word_vectorarray_value a1_ptr a1 ⋆
+          word_vectorarray_value a2_ptr a2 ⋆ R) mem;
+       ensures tr' mem' :=
+         tr' = tr /\
+         let res := vect_memcpy_s len a1 a2 pr1 pr2 in
+         (word_vectorarray_value a1_ptr (fst res) ⋆
+          word_vectorarray_value a2_ptr (snd res) ⋆ R) mem' }.
 
    Derive vect_memcpy_s_body SuchThat
           (defn! "vect_memcpy_s"("len", "a1", "a2") { vect_memcpy_s_body },
@@ -1302,7 +443,174 @@ Section with_parameters.
 
      all: repeat compile_step; compile_done.
    Qed.
-End with_parameters.
+
+   Definition sizedlist_memcpy (len: word)
+           (a1: ListArray.t word)
+           (a2: ListArray.t word) :=
+     let/n from := word.of_Z 0 in
+     let/n step := word.of_Z 1 in
+     let/n a2 := ranged_for_u
+                  from len step
+                  (fun tok idx a2 Hlt =>
+                     let/n v := ListArray.get a1 idx in
+                     let/n a2 := ListArray.put a2 idx v in
+                     (tok, a2)) a2 in
+     (a1, a2).
+
+   Instance spec_of_sizedlist_memcpy : spec_of "sizedlist_memcpy" :=
+     fnspec "sizedlist_memcpy" (len: word) (a1_ptr a2_ptr : address) /
+            {n1} (a1: ListArray.t word)
+            {n2} (a2: ListArray.t word)
+            (pr1: word.unsigned len < Z.of_nat n1)
+            (pr2: word.unsigned len < Z.of_nat n2)
+            R,
+     { requires tr mem :=
+         (word_sizedlistarray_value a1_ptr n1 a1 ⋆
+          word_sizedlistarray_value a2_ptr n2 a2 ⋆ R) mem;
+       ensures tr' mem' :=
+         tr' = tr /\
+         let res := sizedlist_memcpy len a1 a2 in
+         (word_sizedlistarray_value a1_ptr n1 (fst res) ⋆
+          word_sizedlistarray_value a2_ptr n2 (snd res) ⋆ R) mem' }.
+
+   Derive sizedlist_memcpy_body SuchThat
+         (defn! "sizedlist_memcpy"("len", "a1", "a2") { sizedlist_memcpy_body },
+          implements sizedlist_memcpy)
+         As sizedlist_memcpy_correct.
+   Proof.
+     compile_setup.
+
+     repeat compile_step.
+
+     simple apply compile_nlet_as_nlet_eq.
+     eapply compile_ranged_for_u with (loop_pred := (fun idx a2 tr' mem' locals' =>
+         tr' = tr /\
+         locals' = (∅[["len" ← len]][["a1" ← a1_ptr]][["a2" ← a2_ptr]]
+                     [["from" ← idx]][["step" ← word.of_Z 1]]) /\
+         (word_sizedlistarray_value a1_ptr n1 a1 *
+          word_sizedlistarray_value a2_ptr n2 a2 * R)%sep mem')).
+
+     all: repeat compile_step; try lia; compile_done.
+   Qed.
+
+   Definition unsizedlist_memcpy (len: word)
+           (a1: ListArray.t word)
+           (a2: ListArray.t word) :=
+     let/n from := word.of_Z 0 in
+     let/n step := word.of_Z 1 in
+     let/n a2 := ranged_for_u
+                  from len step
+                  (fun tok idx a2 Hlt =>
+                     let/n v := ListArray.get a1 idx in
+                     let/n a2 := ListArray.put a2 idx v in
+                     (tok, a2)) a2 in
+     (a1, a2).
+
+   Instance spec_of_unsizedlist_memcpy : spec_of "unsizedlist_memcpy" :=
+     fnspec "unsizedlist_memcpy" (len: word) (a1_ptr a2_ptr : address) /
+            (a1: ListArray.t word) (a2: ListArray.t word)
+            (pr1: word.unsigned len < Z.of_nat (List.length a1))
+            (pr2: word.unsigned len < Z.of_nat (List.length a2))
+            R,
+     { requires tr mem :=
+         (word_listarray_value a1_ptr a1 ⋆
+          word_listarray_value a2_ptr a2 ⋆ R) mem;
+       ensures tr' mem' :=
+         tr' = tr /\
+         let res := unsizedlist_memcpy len a1 a2 in
+         (word_listarray_value a1_ptr (fst res) ⋆
+          word_listarray_value a2_ptr (snd res) ⋆ R) mem' }.
+
+   Derive unsizedlist_memcpy_body SuchThat
+         (defn! "unsizedlist_memcpy"("len", "a1", "a2") { unsizedlist_memcpy_body },
+          implements unsizedlist_memcpy)
+         As unsizedlist_memcpy_correct.
+   Proof.
+     compile_setup.
+
+     repeat compile_step.
+
+     simple apply compile_nlet_as_nlet_eq.
+     eapply compile_ranged_for_u with (loop_pred := (fun idx a2 tr' mem' locals' =>
+         tr' = tr /\
+         locals' = (∅[["len" ← len]][["a1" ← a1_ptr]][["a2" ← a2_ptr]]
+                     [["from" ← idx]][["step" ← word.of_Z 1]]) /\
+         (word_listarray_value a1_ptr a1 *
+          word_listarray_value a2_ptr a2 * R)%sep mem')).
+
+     (*  FIXME remove previous hints *)
+     (* Import UnsizedListArrayCompiler. *)
+     Hint Extern 1 => simple eapply @compile_word_unsizedlistarray_get; shelve : compiler.
+     Hint Extern 1 => simple eapply @compile_word_unsizedlistarray_put; shelve : compiler.
+
+     all: repeat compile_step; compile_done; unfold id.
+
+     { lia. (* loop index in bounds + function precondition *) }
+     { (* Note the call to induction.
+          Without vectors or the sizedlist predicate, we need to check that the index is in bounds but we modified the array.
+          Using a vector type instead keeps the information in the type and the statement of put specifies that the length is preserved.
+          Putting that info in the representation predicates has a similar effect.
+          Without this, we need to perform induction explicitly. *)
+       subst a.
+       apply ranged_for_u_ind.
+       - lia.
+       - intros; unfold nlet; cbn.
+         rewrite ListArray.put_length.
+         assumption. }
+   Qed.
+
+   Program Definition incr_gallina (c: cell) : cell :=
+     let/n one := word.of_Z 1 in
+     let/n from := word.of_Z 3 in
+     let/n to := word.of_Z 5 in
+     let/n step := word.of_Z 1 in
+     let/n tick := word.of_Z 0 in
+     let/n (tick, c) :=
+        ranged_for_u (A := word * cell)
+                     from to step
+                     (fun tok idx acc bounded =>
+                        let '(tick, c) := acc in
+                        let/n v := get c in
+                        let/n v := word.add v idx in
+                        let/n c := put v c in
+                        let/n tick := word.add tick one in
+                        (tok, (tick, c)))
+                     (tick, c) : word * cell in
+     (let/n v := get c in
+      let/n v := word.add v tick in
+      let/n c := put v c in
+      c).
+
+   Instance spec_of_incr : spec_of "incr" :=
+     fnspec "incr" c_ptr / (c: cell) R,
+     { requires tr mem :=
+         (cell_value c_ptr c ⋆ R) mem;
+       ensures tr' mem' :=
+         tr' = tr /\
+         (cell_value c_ptr (incr_gallina c) ⋆ R) mem' }.
+
+   Derive incr_body SuchThat
+         (defn! "incr"("c") { incr_body },
+          implements incr_gallina)
+         As body_correct.
+   Proof.
+     compile_setup.
+
+     repeat compile_step.
+
+     simple apply compile_nlet_as_nlet_eq.
+     eapply compile_ranged_for_u with (loop_pred := (fun idx acc tr' mem' locals' =>
+         let '(tick, c) := acc in
+         tr' = tr /\
+         (* locals' = map.put locals "tick" tick /\ *)
+         locals' = (∅[["c" ← c_ptr]][["one" ← v]]
+                     [["from" ← idx]][["to" ← v1]][["step" ← v2]]
+                     [["tick" ← tick]]) /\
+         (cell_value c_ptr c * R)%sep mem')).
+
+     all: repeat compile_step; compile_done.
+   Qed.
+End Ex.
 
 (* Require Import bedrock2.NotationsCustomEntry. *)
 (* Require Import bedrock2.NotationsInConstr. *)
