src/Rupicola/Lib/Arrays.v
@@ -1,0 +1,680 @@
+From Coq Require Vector List.
+Require Import Rupicola.Lib.Core.
+Require Import Rupicola.Lib.Notations.
+(* Require Import Arith PeanoNat. *)
+
+Class HasDefault (T: Type) := default: T.
+
+Class Convertible (T1 T2: Type) := cast: T1 -> T2.
+
+Module VectorArray.
+  Section VectorArray.
+    Context {K V: Type}.
+    Context {Conv: Convertible K nat}.
+
+    Definition t n := Vector.t V n.
+    Definition get {n} (a: t n) (k: K) (pr: cast k < n) : V :=
+      Vector.nth_order a pr.
+    Definition put {n} (a: t n) (k: K) (pr: cast k < n) (v: V) : t n :=
+      Vector.replace_order a pr v.
+    (* FIXME needs an accessor that generates a test and returns a default *)
+  End VectorArray.
+
+  Arguments t : clear implicits.
+End VectorArray.
+
+Module ListArray.
+  Section ListArray.
+    Context {K V: Type}.
+    Context {HD: HasDefault V}.
+    Context {Conv: Convertible K nat}.
+
+    Definition t := list V.
+    Definition get (a: t) (k: K) : V :=
+      List.nth (cast k) a default.
+    Definition put (a: t) (k: K) (v: V) : t :=
+      replace_nth (cast k) a v.
+    (* FIXME needs an accessor that generates a test and returns a default *)
+
+    Lemma put_length (a: t) (k: K) (v: V) :
+      List.length (put a k v) = List.length a.
+    Proof. intros; apply replace_nth_length. Qed.
+  End ListArray.
+
+  Arguments t : clear implicits.
+End ListArray.
+
+Section with_parameters.
+  Context {semantics : Semantics.parameters}
+          {semantics_ok : Semantics.parameters_ok semantics}.
+
+  Open Scope Z_scope.
+
+  Section WordArray.
+    Context
+      {A K} (to_list: A -> list word) (to_word: K -> word)
+      (get: A -> K -> word)
+      (put: A -> K -> word -> A)
+      (repr: address -> A -> Semantics.mem -> Prop).
+
+    Notation to_nat idx := (Z.to_nat (word.unsigned (to_word idx))).
+
+    Context (a : A) (a_ptr : word) (a_var : string)
+            (val: word) (val_var: string)
+            (idx : K) (idx_var : string).
+
+    Context
+      (Hget: forall a,
+         exists default,
+           get a idx =
+           List.hd default (List.skipn (to_nat idx) (to_list a)))
+      (Hput:
+         (to_nat idx < List.length (to_list a))%nat ->
+         to_list (put a idx val) =
+         List.app
+           (List.firstn (to_nat idx) (to_list a))
+           (val :: List.skipn (S (to_nat idx)) (to_list a)))
+      (Hgetput:
+         (to_nat idx < List.length (to_list a))%nat ->
+         get (put a idx val) idx = val)
+      (Hrw:
+         Lift1Prop.iff1
+           (repr a_ptr a)
+           (array scalar (word.of_Z (Memory.bytes_per_word Semantics.width))
+                  a_ptr (to_list a)))
+      (Hrw_put:
+         Lift1Prop.iff1
+           (repr a_ptr (put a idx val))
+           (array scalar (word.of_Z (Memory.bytes_per_word Semantics.width))
+                  a_ptr (to_list (put a idx val)))).
+
+    Lemma compile_word_array_get {tr mem locals functions}:
+      let v := get a idx in
+      forall {P} {pred: P v -> predicate} {k: nlet_eq_k P v} {k_impl : cmd}
+        R (var : string),
+
+        (Z.to_nat (word.unsigned (to_word idx)) < Datatypes.length (to_list a))%nat ->
+
+        sep (repr a_ptr a) R mem ->
+        map.get locals a_var = Some a_ptr ->
+        map.get locals idx_var = Some (to_word idx) ->
+
+        (let v := v in
+         <{ Trace := tr;
+            Memory := mem;
+            Locals := map.put locals var v;
+            Functions := functions }>
+         k_impl
+         <{ pred (k v eq_refl) }>) ->
+        <{ Trace := tr;
+           Memory := mem;
+           Locals := locals;
+           Functions := functions }>
+        cmd.seq
+          (cmd.set
+             var
+             (expr.load
+                access_size.word
+                (expr.op bopname.add
+                         (expr.var a_var)
+                         (expr.op bopname.mul
+                                  (expr.literal (Memory.bytes_per_word Semantics.width))
+                                  (expr.var idx_var)))))
+          k_impl
+        <{ pred (nlet_eq [var] v k) }>.
+    Proof.
+      cbn; intros Hlt *.
+      pose proof word.unsigned_range (to_word idx) as (Hge & _).
+      destruct (Hget a) as [default Hget0].
+
+      exists (get a idx); split; cbn; [ | assumption ].
+      exists a_ptr; split; [ eassumption | ]; cbn.
+      exists (to_word idx); split; [ eassumption | ]; cbn.
+      eexists; split; [ | reflexivity ].
+
+      eapply load_word_of_sep.
+      seprewrite_in Hrw H0.        (* FIXME seprewrite shouldn't rename *)
+      (* FIXME: BEDROCK2: Adding an extra "_" at the end shelves an inequality *)
+      once (seprewrite_in open_constr:(array_index_nat_inbounds
+                                         _ _ _ _ (Z.to_nat (word.unsigned (to_word idx)))) H5).
+      { assumption. }
+
+      rewrite word.ring_morph_mul, Z2Nat.id, !word.of_Z_unsigned in H4 by assumption.
+      rewrite Hget0.
+      ecancel_assumption.
+    Qed.
+
+    Lemma compile_word_array_put {tr mem locals functions} :
+      let v := put a idx val in
+      forall {P} {pred: P v -> predicate} {k: nlet_eq_k P v} {k_impl: cmd}
+        R (var: string),
+
+      (Z.to_nat (word.unsigned (to_word idx)) < Datatypes.length (to_list a))%nat ->
+
+      sep (repr a_ptr a) R mem ->
+      map.get locals a_var = Some a_ptr ->
+      map.get locals idx_var = Some (to_word idx) ->
+      map.get locals val_var = Some val ->
+
+      (let v := v in
+       forall mem',
+         sep (repr a_ptr v) R mem' ->
+         <{ Trace := tr;
+            Memory := mem';
+            Locals := locals;
+            Functions := functions }>
+         k_impl
+         <{ pred (k v eq_refl) }>) ->
+      <{ Trace := tr;
+         Memory := mem;
+         Locals := locals;
+         Functions := functions }>
+      cmd.seq
+        (cmd.store
+           access_size.word
+           (expr.op bopname.add
+                    (expr.var a_var)
+                    (expr.op bopname.mul
+                             (expr.literal (Memory.bytes_per_word Semantics.width))
+                             (expr.var idx_var)))
+           (expr.var val_var))
+        k_impl
+      <{ pred (nlet_eq [var] v k) }>.
+    Proof.
+      cbn; intros Hlt *.
+      pose proof word.unsigned_range (to_word idx) as (Hge & _).
+      destruct (Hget (put a idx val)) as [default Hget0].
+      eexists; split; cbn.
+
+      { eexists; split; [ eassumption | ]; cbn.
+        eexists; split; [ eassumption | reflexivity ]. }
+
+      { eexists; split; cbn.
+        { eexists; split; [ eassumption | reflexivity ]. }
+        { seprewrite_in Hrw H0.
+          once (seprewrite_in
+                  open_constr:(array_index_nat_inbounds
+                                 _ _ (default := default) _ _ (Z.to_nat (word.unsigned (to_word idx)))) H6).
+          { assumption. }
+
+          eapply store_word_of_sep.
+          { rewrite word.ring_morph_mul, Z2Nat.id, !word.of_Z_unsigned in H5 by assumption.
+            ecancel_assumption. }
+          { intros m Hm.
+            apply H4.
+            seprewrite Hrw_put.
+            seprewrite
+              open_constr:(array_index_nat_inbounds
+                             _ _ (default := default) _ _ (Z.to_nat (word.unsigned (to_word idx)))).
+            { rewrite Hput by lia.
+              rewrite List.app_length, List.firstn_length_le by lia.
+              cbn [List.length]; rewrite List.length_skipn.
+              lia. }
+            { rewrite <- Hget0, Hgetput by lia.
+              repeat rewrite word.ring_morph_mul, Z2Nat.id, !word.of_Z_unsigned by lia.
+              rewrite Hput by lia.
+
+              rewrite List.firstn_app.
+              rewrite List.firstn_firstn, Min.min_idempotent.
+              rewrite List.firstn_length_le by lia.
+              rewrite Nat.sub_diag; cbn [List.firstn]; rewrite app_nil_r.
+
+              change (val :: ?tl) with (List.app [val] tl).
+              rewrite List.app_assoc, List.skipn_app, List.skipn_all, List.app_nil_l, List.skipn_skipn;
+                rewrite !List.app_length, List.firstn_length_le, (Nat.add_comm _ 1) by lia.
+              - rewrite Nat.sub_diag, Nat.add_0_l.
+                ecancel_assumption.
+              - reflexivity. } } } }
+    Qed.
+  End WordArray.
+
+  Instance Convertible_word_Nat : Convertible word nat :=
+    fun w => Z.to_nat (word.unsigned w).
+  Instance HasDefault_word : HasDefault word :=
+    word.of_Z 0.
+
+  Section WordVectorArray.
+    Definition word_vectorarray_value {n} (addr: address) (a: VectorArray.t word n) : Semantics.mem -> Prop :=
+      array scalar (word.of_Z (Memory.bytes_per_word Semantics.width)) addr (Vector.to_list a).
+
+    Notation repr := word_vectorarray_value.
+    Notation to_list := Vector.to_list.
+    Notation to_word := (proj1_sig (P:=fun idx0 : word => (cast idx0 < _)%nat)).
+    Notation to_nat idx := (Z.to_nat (word.unsigned (to_word idx))).
+
+    Notation get a idx := (VectorArray.get a (proj1_sig idx) (proj2_sig idx)).
+    Notation put a idx v := (VectorArray.put a (proj1_sig idx) (proj2_sig idx) v).
+
+    Lemma WordVectorArray_Hget {n}:
+      forall (a: VectorArray.t word n) idx,
+      exists default,
+        get a idx =
+        List.hd default (List.skipn (to_nat idx) (to_list a)).
+    Proof.
+      intros. exists (word.of_Z 0).
+      apply Vector_nth_hd_skipn.
+      rewrite Fin.to_nat_of_nat; reflexivity.
+    Qed.
+
+    Lemma WordVectorArray_Hput {n} :
+      forall (a : VectorArray.t word n) (idx: {idx : word | (cast idx < n)%nat}) v,
+        to_list (put a idx v) =
+        List.app
+          (List.firstn (to_nat idx) (to_list a))
+          (v :: List.skipn (S (to_nat idx)) (to_list a)).
+    Proof.
+      unfold put.
+      destruct idx as [widx pr]; cbn [proj1_sig proj2_sig].
+      unfold cast, Convertible_word_Nat in *.
+      set (Z.to_nat (word.unsigned widx)) as idx in *.
+      intros.
+      unfold Vector.replace_order; erewrite Vector_to_list_replace by reflexivity.
+      rewrite <- replace_nth_eqn by (rewrite Vector_to_list_length; assumption).
+      rewrite Fin.to_nat_of_nat; reflexivity.
+    Qed.
+
+    Lemma WordVectorArray_Hgetput {n} :
+      forall (a : VectorArray.t word n) (idx: {idx : word | (cast idx < n)%nat}) v,
+        get (put a idx v) idx = v.
+    Proof.
+      unfold get, put, Vector.nth_order, Vector.replace_order.
+      intros; apply Vector_nth_replace.
+    Qed.
+
+    Lemma WordVectorArray_Hrw {n}:
+      forall addr (a: VectorArray.t word n),
+        Lift1Prop.iff1
+          (repr addr a)
+          (array scalar (word.of_Z (Memory.bytes_per_word Semantics.width))
+                 addr (to_list a)).
+    Proof. reflexivity. Qed.
+
+    Lemma compile_word_vectorarray_get {n} {tr mem locals functions}
+          (a: VectorArray.t word n) idx pr:
+      let v := VectorArray.get a idx pr in
+      forall {P} {pred: P v -> predicate} {k: nlet_eq_k P v} {k_impl}
+        R (a_ptr: address) a_var idx_var var,
+
+        sep (word_vectorarray_value a_ptr a) R mem ->
+        map.get locals a_var = Some a_ptr ->
+        map.get locals idx_var = Some idx ->
+
+        (let v := v in
+         <{ Trace := tr;
+            Memory := mem;
+            Locals := map.put locals var v;
+            Functions := functions }>
+         k_impl
+         <{ pred (k v eq_refl) }>) ->
+        <{ Trace := tr;
+           Memory := mem;
+           Locals := locals;
+           Functions := functions }>
+        cmd.seq
+          (cmd.set
+             var
+             (expr.load
+                access_size.word
+                (expr.op bopname.add
+                         (expr.var a_var)
+                         (expr.op bopname.mul
+                                  (expr.literal (Memory.bytes_per_word Semantics.width))
+                                  (expr.var idx_var)))))
+          k_impl
+        <{ pred (nlet_eq [var] v k) }>.
+    Proof.
+      intros.
+      change v with
+          ((fun a idx => VectorArray.get a (proj1_sig idx) (proj2_sig idx))
+             a (exist (fun idx => cast idx < n)%nat idx pr)).
+      eapply (compile_word_array_get to_list to_word);
+        eauto using WordVectorArray_Hget, WordVectorArray_Hrw.
+      { rewrite Vector_to_list_length.
+        simpl. assumption. }
+    Qed.
+
+    Lemma compile_word_vectorarray_put {n} {tr mem locals functions}
+          (a: VectorArray.t word n) idx pr val:
+      let v := VectorArray.put a idx pr val in
+      forall {P} {pred: P v -> predicate} {k: nlet_eq_k P v} {k_impl}
+        R a_ptr a_var idx_var val_var var,
+
+        sep (word_vectorarray_value a_ptr a) R mem ->
+        map.get locals a_var = Some a_ptr ->
+        map.get locals idx_var = Some idx ->
+        map.get locals val_var = Some val ->
+
+        (let v := v in
+         forall mem',
+           sep (word_vectorarray_value a_ptr v) R mem' ->
+           <{ Trace := tr;
+              Memory := mem';
+              Locals := locals;
+              Functions := functions }>
+           k_impl
+           <{ pred (k v eq_refl) }>) ->
+        <{ Trace := tr;
+           Memory := mem;
+           Locals := locals;
+           Functions := functions }>
+        cmd.seq
+          (cmd.store
+             access_size.word
+             (expr.op bopname.add
+                      (expr.var a_var)
+                      (expr.op bopname.mul
+                               (expr.literal (Memory.bytes_per_word Semantics.width))
+                               (expr.var idx_var)))
+             (expr.var val_var))
+          k_impl
+        <{ pred (nlet_eq [var] v k) }>.
+    Proof.
+      intros.
+      change v with
+          ((fun v idx val => VectorArray.put a (proj1_sig idx) (proj2_sig idx) val)
+             v (exist (fun idx => cast idx < n)%nat idx pr) val).
+      eapply (compile_word_array_put
+                to_list to_word
+                (fun a idx => get a idx)
+                (fun a idx v => put a idx v));
+        eauto using WordVectorArray_Hget, WordVectorArray_Hrw,
+        WordVectorArray_Hgetput, WordVectorArray_Hput.
+      rewrite Vector_to_list_length; assumption.
+    Qed.
+  End WordVectorArray.
+
+  Section WordListArray.
+    Definition word_listarray_value (addr: address) (a: ListArray.t word)
+      : Semantics.mem -> Prop :=
+      array scalar (word.of_Z (Memory.bytes_per_word Semantics.width)) addr a.
+
+    Notation repr := word_listarray_value.
+    Notation to_list x := x (only parsing).
+    Notation to_word x := x (only parsing).
+    Notation to_nat idx := (Z.to_nat (word.unsigned (to_word idx))).
+
+    Notation get a idx := (ListArray.get a idx).
+    Notation put a idx v := (ListArray.put a idx v).
+
+    Lemma WordListArray_Hget:
+      forall (a: ListArray.t word) idx,
+      exists default,
+        get a idx =
+        List.hd default (List.skipn (to_nat idx) (to_list a)).
+    Proof.
+      intros. exists (word.of_Z 0).
+      unfold get; rewrite <- List.nth_default_eq.
+      apply List.hd_skipn_nth_default.
+    Qed.
+
+    Lemma WordListArray_Hput :
+      forall (a : ListArray.t word) (idx: word) v,
+        (to_nat idx < Datatypes.length a)%nat ->
+        to_list (put a idx v) =
+        List.app
+          (List.firstn (to_nat idx) (to_list a))
+          (v :: List.skipn (S (to_nat idx)) (to_list a)).
+    Proof.
+      unfold put; eauto using replace_nth_eqn.
+    Qed.
+
+    Lemma WordListArray_Hgetput :
+      forall (a : ListArray.t word) (idx: word) v,
+        (to_nat idx < Datatypes.length a)%nat ->
+        get (put a idx v) idx = v.
+    Proof.
+      unfold get, put.
+      intros; apply nth_replace_nth; (assumption || reflexivity).
+    Qed.
+
+    Lemma WordListArray_Hrw:
+      forall addr (a: ListArray.t word),
+        Lift1Prop.iff1
+          (repr addr a)
+          (array scalar (word.of_Z (Memory.bytes_per_word Semantics.width))
+                 addr (to_list a)).
+    Proof. reflexivity. Qed.
+
+    Lemma compile_word_unsizedlistarray_get {tr mem locals functions}
+          (a: ListArray.t word) idx:
+      let v := ListArray.get a idx in
+      forall {P} {pred: P v -> predicate} {k: nlet_eq_k P v} {k_impl}
+        R (a_ptr: address) a_var idx_var var,
+
+        sep (word_listarray_value a_ptr a) R mem ->
+        map.get locals a_var = Some a_ptr ->
+        map.get locals idx_var = Some idx ->
+
+        word.unsigned idx < Z.of_nat (Datatypes.length (id a)) ->
+
+        (let v := v in
+         <{ Trace := tr;
+            Memory := mem;
+            Locals := map.put locals var v;
+            Functions := functions }>
+         k_impl
+         <{ pred (k v eq_refl) }>) ->
+        <{ Trace := tr;
+           Memory := mem;
+           Locals := locals;
+           Functions := functions }>
+        cmd.seq
+          (cmd.set
+             var
+             (expr.load
+                access_size.word
+                (expr.op bopname.add
+                         (expr.var a_var)
+                         (expr.op bopname.mul
+                                  (expr.literal (Memory.bytes_per_word Semantics.width))
+                                  (expr.var idx_var)))))
+          k_impl
+        <{ pred (nlet_eq [var] v k) }>.
+    Proof.
+      intros.
+      eapply (compile_word_array_get id id);
+        eauto using WordListArray_Hget, WordListArray_Hrw.
+      pose proof word.unsigned_range idx.
+      unfold id in *; lia.
+    Qed.
+
+    Lemma compile_word_unsizedlistarray_put {tr mem locals functions}
+          (a: ListArray.t word) idx val:
+      let v := ListArray.put a idx val in
+      forall {P} {pred: P v -> predicate} {k: nlet_eq_k P v} {k_impl}
+        R (a_ptr: address) a_var idx_var val_var var,
+
+        sep (word_listarray_value a_ptr a) R mem ->
+        map.get locals a_var = Some a_ptr ->
+        map.get locals idx_var = Some idx ->
+        map.get locals val_var = Some val ->
+
+        (word.unsigned idx < Z.of_nat (List.length a))%Z ->
+
+        (let v := v in
+         forall mem',
+           sep (word_listarray_value a_ptr v) R mem' ->
+           <{ Trace := tr;
+              Memory := mem';
+              Locals := locals;
+              Functions := functions }>
+           k_impl
+           <{ pred (k v eq_refl) }>) ->
+        <{ Trace := tr;
+           Memory := mem;
+           Locals := locals;
+           Functions := functions }>
+        cmd.seq
+          (cmd.store
+             access_size.word
+             (expr.op bopname.add
+                      (expr.var a_var)
+                      (expr.op bopname.mul
+                               (expr.literal (Memory.bytes_per_word Semantics.width))
+                               (expr.var idx_var)))
+             (expr.var val_var))
+          k_impl
+        <{ pred (nlet_eq [var] v k) }>.
+    Proof.
+      intros.
+      eapply (compile_word_array_put id id);
+        eauto using WordListArray_Hget, WordListArray_Hput,
+        WordListArray_Hgetput, WordListArray_Hrw.
+      unfold id; pose proof word.unsigned_range idx.
+      lia.
+    Qed.
+  End WordListArray.
+
+  Section WordSizedListArray.
+    Definition word_sizedlistarray_value (addr: address) (len: nat) (a: ListArray.t word)
+      : Semantics.mem -> Prop :=
+      sep (emp (List.length a = len)) (array scalar (word.of_Z (Memory.bytes_per_word Semantics.width)) addr a).
+
+    Notation repr := word_sizedlistarray_value.
+    Notation to_list x := x (only parsing).
+    Notation to_word x := x (only parsing).
+    Notation to_nat idx := (Z.to_nat (word.unsigned (to_word idx))).
+
+    Notation get a idx := (ListArray.get a idx).
+    Notation put a idx v := (ListArray.put a idx v).
+
+    Lemma WordSizedListArray_Hrw:
+      forall addr sz (a: ListArray.t word),
+        List.length a = sz ->
+        Lift1Prop.iff1
+          (repr addr sz a)
+          (array scalar (word.of_Z (Memory.bytes_per_word Semantics.width))
+                 addr (to_list a)).
+    Proof.
+      unfold word_sizedlistarray_value.
+      red; intros; rewrite sep_emp_l; tauto.
+    Qed.
+
+    Lemma WordSizedListArray_length :
+      forall addr sz (a: ListArray.t word) mem R,
+        (repr addr sz a * R)%sep mem -> List.length a = sz.
+    Proof.
+      intros * H; unfold repr in H.
+      eapply proj1. apply sep_emp_l with (m := mem).
+      ecancel_assumption.
+    Qed.
+
+    Lemma compile_word_sizedlistarray_get {sz} {tr mem locals functions}
+          (a: ListArray.t word) idx:
+      let v := ListArray.get a idx in
+      forall {P} {pred: P v -> predicate} {k: nlet_eq_k P v} {k_impl}
+        R (a_ptr: address) a_var idx_var var,
+
+        sep (word_sizedlistarray_value a_ptr sz a) R mem ->
+        map.get locals a_var = Some a_ptr ->
+        map.get locals idx_var = Some idx ->
+
+        word.unsigned idx < Z.of_nat sz ->
+
+        (let v := v in
+         <{ Trace := tr;
+            Memory := mem;
+            Locals := map.put locals var v;
+            Functions := functions }>
+         k_impl
+         <{ pred (k v eq_refl) }>) ->
+        <{ Trace := tr;
+           Memory := mem;
+           Locals := locals;
+           Functions := functions }>
+        cmd.seq
+          (cmd.set
+             var
+             (expr.load
+                access_size.word
+                (expr.op bopname.add
+                         (expr.var a_var)
+                         (expr.op bopname.mul
+                                  (expr.literal (Memory.bytes_per_word Semantics.width))
+                                  (expr.var idx_var)))))
+          k_impl
+        <{ pred (nlet_eq [var] v k) }>.
+    Proof.
+      intros.
+      eapply (compile_word_array_get id id _ (fun addr a => repr addr sz a));
+        eauto using WordListArray_Hget.
+      - eapply WordSizedListArray_Hrw, WordSizedListArray_length.
+        eassumption.
+      - unfold id.
+        erewrite WordSizedListArray_length by eassumption.
+        pose proof word.unsigned_range idx.
+        lia.
+    Qed.
+
+    Lemma compile_word_sizedlistarray_put {sz} {tr mem locals functions}
+          (a: ListArray.t word) idx val:
+      let v := ListArray.put a idx val in
+      forall {P} {pred: P v -> predicate} {k: nlet_eq_k P v} {k_impl}
+        R (a_ptr: address) a_var idx_var val_var var,
+
+        sep (word_sizedlistarray_value a_ptr sz a) R mem ->
+        map.get locals a_var = Some a_ptr ->
+        map.get locals idx_var = Some idx ->
+        map.get locals val_var = Some val ->
+
+        (word.unsigned idx < Z.of_nat sz)%Z ->
+
+        (let v := v in
+         forall mem',
+           sep (word_sizedlistarray_value a_ptr sz v) R mem' ->
+           <{ Trace := tr;
+              Memory := mem';
+              Locals := locals;
+              Functions := functions }>
+           k_impl
+           <{ pred (k v eq_refl) }>) ->
+        <{ Trace := tr;
+           Memory := mem;
+           Locals := locals;
+           Functions := functions }>
+        cmd.seq
+          (cmd.store
+             access_size.word
+             (expr.op bopname.add
+                      (expr.var a_var)
+                      (expr.op bopname.mul
+                               (expr.literal (Memory.bytes_per_word Semantics.width))
+                               (expr.var idx_var)))
+             (expr.var val_var))
+          k_impl
+        <{ pred (nlet_eq [var] v k) }>.
+    Proof.
+      intros.
+      eapply (compile_word_array_put id id _ _ (fun (addr: word) a => repr addr sz a));
+        eauto using WordListArray_Hget, WordListArray_Hput,
+        WordListArray_Hgetput.
+      - eapply WordSizedListArray_Hrw, WordSizedListArray_length.
+        eassumption.
+      - eapply WordSizedListArray_Hrw.
+        unfold id; rewrite ListArray.put_length.
+        eapply WordSizedListArray_length.
+        eassumption.
+      - unfold id; pose proof word.unsigned_range idx.
+        erewrite WordSizedListArray_length by eassumption.
+        lia.
+    Qed.
+  End WordSizedListArray.
+End with_parameters.
+
+Module VectorArrayCompiler.
+  Hint Extern 1 => simple eapply @compile_word_vectorarray_get; shelve : compiler.
+  Hint Extern 1 => simple eapply @compile_word_vectorarray_put; shelve : compiler.
+End VectorArrayCompiler.
+
+Module UnsizedListArrayCompiler.
+  Hint Extern 1 => simple eapply @compile_word_unsizedlistarray_get; shelve : compiler.
+  Hint Extern 1 => simple eapply @compile_word_unsizedlistarray_put; shelve : compiler.
+End UnsizedListArrayCompiler.
+
+Module SizedListArrayCompiler.
+  Hint Extern 1 => simple eapply @compile_word_sizedlistarray_get; shelve : compiler.
+  Hint Extern 1 => simple eapply @compile_word_sizedlistarray_put; shelve : compiler.
+End SizedListArrayCompiler.
+
+Export VectorArrayCompiler.
+(* UnsizedListArrayCompiler and SizedListArrayCompiler conflict, so don't export them. *)
